Tests/UIDEquivSpec.lean
@@ -1,0 +1,57 @@
+import «Lp2lc».Active.Util
+
+namespace Tests.UIDEquivSpec
+
+open Lp2lc.Active.Util
+open UIDEquiv
+
+def group : UIDEquiv Nat Nat where
+  getUID := id
+  inv := id
+  leftInv := by
+    intro value
+    rfl
+  rightInv := by
+    intro id
+    rfl
+
+@[reducible] def boolMetadata : Aux group (λ _value => Bool) where
+  Evidence := λ _id => Bool
+  lookup := λ _id => none
+  saveMeta := λ bundle => bundle.snd
+  loadMeta := λ id2 => id2.snd
+
+@[reducible] def unitMetadata : Aux group (λ _value => Unit) where
+  Evidence := λ _id => Unit
+  lookup := λ _id => none
+  saveMeta := λ bundle => bundle.snd
+  loadMeta := λ id2 => id2.snd
+
+section getUID
+
+example :
+    boolMetadata.Evidence (group.getUID 1) :=
+  boolMetadata.saveMeta ⟨1, true⟩
+
+example :
+    boolMetadata.Evidence (group.getUID 1) ×
+      unitMetadata.Evidence (group.getUID 1) :=
+  ⟨boolMetadata.saveMeta ⟨1, true⟩,
+    unitMetadata.saveMeta ⟨1, ()⟩⟩
+
+example :
+    group.inv (group.getUID 1) = 1 := by
+  exact boolMetadata.leftInvValue ⟨1, true⟩
+
+example :
+    boolMetadata.loadMeta
+      ⟨group.getUID 1, boolMetadata.saveMeta ⟨1, true⟩⟩ = true := by
+  rfl
+
+example :
+    boolMetadata.lookup (group.getUID 1) = none := by
+  rfl
+
+end getUID
+
+end Tests.UIDEquivSpec
